dnsprotect/cleanup/lucidBase4.dfy
@@ -29,6 +29,241 @@ Changes [5-12-2024]
 12.add "Parse" module and parser to verify
 -------------------------------------------------------------------------*/
 
+
+abstract module LucidBase {
+   import opened Types
+
+   type Event (==)
+   datatype TimedEvent = 
+      TimedEvent (event: Event, ghost time: nat, timestamp: uint8)
+            
+   datatype RecircCmd = RecircCmd (generate: bool, event: Event)
+
+   datatype GeneratedEvent = Event(event:Event, ports : set<uint8>)
+
+   // system state that can be _read_ by the program, 
+   // but may not be _modified_ by the program, or 
+   // read by toplevel predicates. 
+   class Sys {
+      static const T : uint16 := 256          // number must match limit on timestamp
+      ghost var time : nat
+      ghost var lastTime : nat
+      var timestamp : uint8
+      var queue : seq <TimedEvent>
+
+      constructor ()
+      ensures fresh(this)
+      ensures validQueue(queue)
+       {
+         time := 0;
+         lastTime := 0;
+         timestamp := 0;
+         queue := [];
+      }
+
+      ghost predicate validQueue (q: seq <TimedEvent>)   // queue invariant
+      // In a valid queue, times and timestamps match, and time is
+      // nondecreasing.
+      {
+         match |q| {
+            case 0 => true
+            case _ =>
+            (  (  forall j | 0 <= j <= |q|-1 ::
+                     q[j].timestamp == q[j].time % T  )
+            && (  forall j | 0 <= j < |q|-1 ::
+                     q[j].time <= q[j+1].time  )      )  }
+      } 
+   }
+
+   class Interpreter {
+      // The interpreter is for running a program.
+      var prog : Program
+      var sys : Sys
+      constructor (p : Program)
+         ensures fresh(this)
+         ensures sys == prog.sys
+         {
+            prog := p;
+            sys := p.sys;
+         }
+
+      method simulateArrival (q: seq <TimedEvent>)
+      // This method adds zero or more events to the queue.
+         modifies sys`queue
+         requires sys.validQueue (sys.queue)
+         requires q == sys.queue
+         ensures q <= sys.queue           // old queue is a prefix of new queue
+         ensures sys.validQueue (sys.queue)
+
+      method pickNextEvent (q: seq <TimedEvent>)
+         modifies sys, sys`lastTime, prog`generatedEvents, prog
+         modifies prog.globals
+         requires prog.sys == this.sys
+         requires prog.generatedEvents == {}
+         requires sys.validQueue (sys.queue)
+         requires |sys.queue| > 0
+         requires q == sys.queue
+         requires prog.globals.parameterConstraints ()
+         requires prog.globals.stateInvariant (q[0].time, q[0].timestamp, sys.lastTime)
+         requires (sys.time == q[0].time && sys.timestamp == q[0].timestamp) <==> prog.globals.stateInvariant (q[0].time , q[0].timestamp, sys.lastTime)
+         requires prog.operatingAssumptions (q[0].event, q[0].time, q[0].timestamp, sys.lastTime)
+         ensures sys.validQueue (sys.queue)
+         ensures ( |sys.queue| == |q| - 1 ) || ( |sys.queue| == |q| )
+         ensures prog.sys == this.sys
+      { 
+         assert prog.globals.stateInvariant (q[0].time, q[0].timestamp, sys.lastTime);
+         sys.time := q[0].time;
+         sys.timestamp := q[0].timestamp;
+         assert prog.globals.stateInvariant (sys.time, q[0].timestamp, sys.lastTime);
+
+         // sys.timestamp := q[0].timestamp;         
+         prog.dispatch(q[0].event);
+         sys.lastTime := 0;
+         // if an event for recirculation was generated, add it to the queue
+         sys.queue := q;
+         assert |sys.queue| > 0;
+         while |prog.generatedEvents| > 0
+            modifies prog`generatedEvents
+            modifies sys`queue
+            invariant |sys.queue| > 0
+            invariant sys.validQueue(sys.queue)
+         {
+            assert |sys.queue| > 0;
+            var generatedEvent :| generatedEvent in prog.generatedEvents;
+            if (generatedEvent.ports == {}) { // recirc event, add to queue
+               var recircEvent: TimedEvent := generateRecircEvent(generatedEvent.event);
+               sys.queue := sys.queue + [recircEvent];
+            }
+            prog.generatedEvents := prog.generatedEvents - {generatedEvent};
+         }
+         sys.queue := q[1..];
+         // lastTime := q[0].time; 
+         sys.lastTime := q[0].time;
+      }
+
+      method generateRecircEvent (e: Event) returns 
+                                                  (recircEvent: TimedEvent)
+         requires sys.validQueue (sys.queue)
+         requires |sys.queue| > 0              // because method is called just
+                    // after dispatch, when dispatched event still in queue
+         ensures recircEvent.time > sys.queue[|sys.queue|-1].time
+         ensures recircEvent.timestamp == recircEvent.time % sys.T
+         ensures unchanged(this`sys)
+      {
+         var recircTimestamp: uint8;
+         recircTimestamp := (sys.queue[|sys.queue|-1].timestamp + 1) % sys.T;
+         recircEvent := 
+                   TimedEvent(e, sys.queue[|sys.queue|-1].time+1, recircTimestamp);
+      }
+
+   }
+
+   class Globals {
+      constructor ()
+         ensures fresh(this)
+
+      ghost predicate stateInvariant (time: nat, timestamp: uint8, lastTime : nat)  
+         reads this
+      ghost predicate parameterConstraints ()          // define in program
+
+
+   }
+
+   class Program {
+      var sys : Sys
+      var globals : Globals
+      var generatedEvents : set<GeneratedEvent>  // the event generated for recirc
+
+      // ghost predicate parameterConstraints ()          // define in program
+      //    reads {this} - {sys}
+      // ghost predicate stateInvariant (time: nat, timestamp: uint8, lastTime:nat)
+      //    reads {this} - {sys}                                    // define in program
+      ghost predicate operatingAssumptions (event: Event, time : nat, timestamp: uint8, lastTime:nat)     
+         reads this`globals, this.globals
+
+      constructor ()                                   // define in program
+         ensures sys.validQueue (sys.queue)
+         ensures fresh(sys)
+         ensures fresh(globals)
+         ensures fresh(this)
+         {
+            sys := new Sys();
+            globals := new Globals();
+         }
+
+      method dispatch (e: Event)
+         modifies globals                                          // define in program
+         modifies this`generatedEvents
+         requires sys.timestamp == sys.time % sys.T
+         requires globals.parameterConstraints ()
+         requires globals.stateInvariant (sys.time, sys.timestamp, sys.lastTime)
+         requires operatingAssumptions (e, sys.time, sys.timestamp, sys.lastTime)
+         requires generatedEvents == {}
+         ensures unchanged(this`sys)
+
+      method generate(e : Event)            // generate recirculation event
+         modifies this`generatedEvents
+      {
+         generatedEvents := generatedEvents + {Event(e, {})};
+      }
+      method generate_port(p : uint8, e : Event)  // generate output event
+         modifies this`generatedEvents
+      {
+         generatedEvents := generatedEvents + {Event(e, {p})};
+      }
+
+   }
+
+   import opened ParseUtils
+   class Parser {
+      static ghost predicate validPacket(p:Packet) 
+      static ghost predicate parserSpecification(p : Packet, d : ParseDecision<Event>) 
+         requires validPacket(p)
+      static function parse(p : Packet) : ParseDecision<Event>
+         requires p.offset == 0
+         requires validPacket(p) 
+         ensures (parserSpecification(p, parse(p)))
+   } 
+
+}
+
+
+module Memop { 
+   type memcalc<!t> = (t, t) -> t
+
+   datatype StateVar<t> = Atomic (val: t)
+
+   method Get<t> (s:StateVar<t>, mget: memcalc, garg: t) returns (oldVal:t)
+   ensures oldVal == mget(s.val, garg)
+   {
+      oldVal := mget (s.val, garg);
+   }
+
+   method Set<t> (s: StateVar<t>, mset: memcalc, sarg: t)
+                                              returns (newVal: StateVar<t>)
+   ensures newVal.val == mset(s.val, sarg)
+   {
+      newVal := Atomic (mset (s.val, sarg));
+      // must be called so that s := newVal;
+   }
+
+   method GetSet<t> (s: StateVar<t>, mget: memcalc, garg: t,
+                                     mset: memcalc, sarg: t)
+                                   returns (oldVal: t, newVal: StateVar<t>)
+   ensures oldVal == mget(s.val, garg)
+   ensures newVal.val == mset(s.val, sarg)
+   {
+      oldVal := mget (s.val, garg);
+      newVal := Atomic (mset (s.val, sarg));
+      // must be called so that s := newVal;
+   }
+
+   // generic memcalcs
+   function nocalc<t> (oldVal: t, newArg: t) : t {  oldVal  }
+   function swapcalc<t> (oldVal: t, newArg: t) : t {  newArg  }
+}
+
+
 module Types {
    // Integer types to use in executable code
    type uint8 = x : nat | 0 <= x < 256
@@ -124,228 +359,4 @@ module ParseUtils {
       (x % 256) as uint8
    }
 
-}
-
-abstract module LucidBase {
-   import opened Types
-
-   type Event (==)
-   datatype TimedEvent = 
-      TimedEvent (event: Event, ghost time: nat, timestamp: uint8)
-            
-   datatype RecircCmd = RecircCmd (generate: bool, event: Event)
-
-   datatype GeneratedEvent = Event(event:Event, ports : set<uint8>)
-
-   // system state that can be _read_ by the program, 
-   // but may not be _modified_ by the program, or 
-   // read by toplevel predicates. 
-   class Sys {
-      static const T : uint16 := 256          // number must match limit on timestamp
-      ghost var time : nat
-      ghost var lastTime : nat
-      var timestamp : uint8
-      var queue : seq <TimedEvent>
-
-      constructor ()
-      ensures fresh(this)
-      ensures validQueue(queue)
-       {
-         time := 0;
-         lastTime := 0;
-         timestamp := 0;
-         queue := [];
-      }
-
-      ghost predicate validQueue (q: seq <TimedEvent>)   // queue invariant
-      // In a valid queue, times and timestamps match, and time is
-      // nondecreasing.
-      {
-         match |q| {
-            case 0 => true
-            case _ =>
-            (  (  forall j | 0 <= j <= |q|-1 ::
-                     q[j].timestamp == q[j].time % T  )
-            && (  forall j | 0 <= j < |q|-1 ::
-                     q[j].time <= q[j+1].time  )      )  }
-      } 
-   }
-
-   class Interpreter {
-      // The interpreter is for running a program.
-      var prog : Program
-      var sys : Sys
-      constructor (p : Program)
-         ensures fresh(this)
-         ensures sys == prog.sys
-         {
-            prog := p;
-            sys := p.sys;
-         }
-
-      method simulateArrival (q: seq <TimedEvent>)
-      // This method adds zero or more events to the queue.
-         modifies sys`queue
-         requires sys.validQueue (sys.queue)
-         requires q == sys.queue
-         ensures q <= sys.queue           // old queue is a prefix of new queue
-         ensures sys.validQueue (sys.queue)
-
-      method pickNextEvent (q: seq <TimedEvent>)
-         modifies sys, sys`lastTime, prog`generatedEvents, prog
-         requires prog.sys == this.sys
-         requires prog.generatedEvents == {}
-         requires sys.validQueue (sys.queue)
-         requires |sys.queue| > 0
-         requires q == sys.queue
-         requires prog.parameterConstraints ()
-         requires prog.stateInvariant (q[0].time, q[0].timestamp, sys.lastTime)
-         requires (sys.time == q[0].time && sys.timestamp == q[0].timestamp) <==> prog.stateInvariant (q[0].time , q[0].timestamp, sys.lastTime)
-         requires prog.operatingAssumptions (q[0].event, q[0].time, q[0].timestamp, sys.lastTime)
-         ensures sys.validQueue (sys.queue)
-         ensures ( |sys.queue| == |q| - 1 ) || ( |sys.queue| == |q| )
-         ensures prog.sys == this.sys
-      { 
-         assert prog.stateInvariant (q[0].time, q[0].timestamp, sys.lastTime);
-         sys.time := q[0].time;
-         sys.timestamp := q[0].timestamp;
-         assert prog.stateInvariant (sys.time, q[0].timestamp, sys.lastTime);
-
-         // sys.timestamp := q[0].timestamp;         
-         prog.dispatch(q[0].event);
-         sys.lastTime := 0;
-         // if an event for recirculation was generated, add it to the queue
-         sys.queue := q;
-         assert |sys.queue| > 0;
-         while |prog.generatedEvents| > 0
-            modifies prog`generatedEvents
-            modifies sys`queue
-            invariant |sys.queue| > 0
-            invariant sys.validQueue(sys.queue)
-         {
-            assert |sys.queue| > 0;
-            var generatedEvent :| generatedEvent in prog.generatedEvents;
-            if (generatedEvent.ports == {}) { // recirc event, add to queue
-               var recircEvent: TimedEvent := generateRecircEvent(generatedEvent.event);
-               sys.queue := sys.queue + [recircEvent];
-            }
-            prog.generatedEvents := prog.generatedEvents - {generatedEvent};
-         }
-         sys.queue := q[1..];
-         // lastTime := q[0].time; 
-         sys.lastTime := q[0].time;
-      }
-
-      method generateRecircEvent (e: Event) returns 
-                                                  (recircEvent: TimedEvent)
-         requires sys.validQueue (sys.queue)
-         requires |sys.queue| > 0              // because method is called just
-                    // after dispatch, when dispatched event still in queue
-         ensures recircEvent.time > sys.queue[|sys.queue|-1].time
-         ensures recircEvent.timestamp == recircEvent.time % sys.T
-         ensures unchanged(this`sys)
-      {
-         var recircTimestamp: uint8;
-         recircTimestamp := (sys.queue[|sys.queue|-1].timestamp + 1) % sys.T;
-         recircEvent := 
-                   TimedEvent(e, sys.queue[|sys.queue|-1].time+1, recircTimestamp);
-      }
-
-   }
-
-   class Program {
-      var sys : Sys
-
-      ghost predicate parameterConstraints ()          // define in program
-         reads {this} - {sys}
-      ghost predicate stateInvariant (time: nat, timestamp: uint8, lastTime:nat)
-         reads {this} - {sys}                                    // define in program
-
-      ghost predicate operatingAssumptions (event: Event, time : nat, timestamp: uint8, lastTime:nat)     
-         reads {this} - {sys}                                        // define in program
-
-      constructor ()                                   // define in program
-         ensures sys.validQueue (sys.queue)
-         // ensures parameterConstraints () // problem: how can the constructor ever ensure this?
-         ensures fresh(sys)
-         ensures fresh(this)
-         {
-            sys := new Sys();
-         }
-
-      method dispatch (e: Event)
-         modifies {this} - {this.sys}                                // define in program
-         requires sys.timestamp == sys.time % sys.T
-         requires parameterConstraints ()
-         requires stateInvariant (sys.time, sys.timestamp, sys.lastTime)
-         requires operatingAssumptions (e, sys.time, sys.timestamp, sys.lastTime)
-         requires generatedEvents == {}
-         ensures unchanged(this`sys)
-
-
-      var generatedEvents : set<GeneratedEvent>  // the event generated for recirc
-
-      method generate(e : Event)            // generate recirculation event
-         modifies this`generatedEvents
-         ensures unchanged(this`sys)
-      {
-         generatedEvents := generatedEvents + {Event(e, {})};
-      }
-      method generate_port(p : uint8, e : Event)  // generate output event
-         modifies this`generatedEvents
-         ensures unchanged(this.sys)
-
-      {
-         generatedEvents := generatedEvents + {Event(e, {p})};
-      }
-
-   }
-
-   import opened ParseUtils
-   class Parser {
-      static ghost predicate validPacket(p:Packet) 
-      static ghost predicate parserSpecification(p : Packet, d : ParseDecision<Event>) 
-         requires validPacket(p)
-      static function parse(p : Packet) : ParseDecision<Event>
-         requires p.offset == 0
-         requires validPacket(p) 
-         ensures (parserSpecification(p, parse(p)))
-   } 
-
-}
-
-
-module Memop { 
-   type memcalc<!t> = (t, t) -> t
-
-   datatype StateVar<t> = Atomic (val: t)
-
-   method Get<t> (s:StateVar<t>, mget: memcalc, garg: t) returns (oldVal:t)
-   ensures oldVal == mget(s.val, garg)
-   {
-      oldVal := mget (s.val, garg);
-   }
-
-   method Set<t> (s: StateVar<t>, mset: memcalc, sarg: t)
-                                              returns (newVal: StateVar<t>)
-   ensures newVal.val == mset(s.val, sarg)
-   {
-      newVal := Atomic (mset (s.val, sarg));
-      // must be called so that s := newVal;
-   }
-
-   method GetSet<t> (s: StateVar<t>, mget: memcalc, garg: t,
-                                     mset: memcalc, sarg: t)
-                                   returns (oldVal: t, newVal: StateVar<t>)
-   ensures oldVal == mget(s.val, garg)
-   ensures newVal.val == mset(s.val, sarg)
-   {
-      oldVal := mget (s.val, garg);
-      newVal := Atomic (mset (s.val, sarg));
-      // must be called so that s := newVal;
-   }
-
-   // generic memcalcs
-   function nocalc<t> (oldVal: t, newArg: t) : t {  oldVal  }
-   function swapcalc<t> (oldVal: t, newArg: t) : t {  newArg  }
 }
